add separation logic libs

WebAssembly/Wasm_Interpreter_Monad_Properties.thy
@@ -1,2 +1,66 @@
-theory Wasm_Interpreter_Monad_Properties imports Wasm_Interpreter_Monad begin
+theory Wasm_Interpreter_Monad_Properties imports "../libs/List_Assn" Wasm_Interpreter_Monad begin
+
+term app_s_f_v_s_mem_size_m
+term app_s_f_v_s_mem_size
+
+definition "mem_m_assn \<equiv> \<lambda>(mr,mm) (mri,mmi). mri \<mapsto>\<^sub>a Rep_mem_rep mr * \<up>(mmi=mm)"
+
+definition "inst_m_assn i ii \<equiv> 
+    inst_m.types ii \<mapsto>\<^sub>a inst.types i
+  * inst_m.funcs ii \<mapsto>\<^sub>a inst.funcs i  
+  * inst_m.tabs  ii \<mapsto>\<^sub>a inst.tabs  i 
+  * inst_m.mems  ii \<mapsto>\<^sub>a inst.mems  i 
+  * inst_m.globs ii \<mapsto>\<^sub>a inst.globs i"
+     
+lemma [sep_heap_rules]: "<mem_m_assn m mi> Array.len (fst mi) <\<lambda>r. mem_m_assn m mi * \<up>(r=length (Rep_mem_rep (fst m)))>"
+  unfolding mem_m_assn_def
+  by (sep_auto split: prod.splits)
+
+method extract_list_idx for i :: nat =
+  (subst listI_assn_extract[of i], (simp;fail), (simp;fail))
+  
+method reinsert_list_idx for i :: nat =
+  rule listI_assn_reinsert[where i=i] listI_assn_reinsert'[where i=i],
+  (frame_inference; fail),
+  (simp;fail),
+  (simp;fail)
+  
+lemma "< mi \<mapsto>\<^sub>a mis * (list_assn mem_m_assn) ms mis * inst_m_assn (f_inst i) ii > 
+    app_s_f_v_s_mem_size_m mi ii vs 
+  <\<lambda>r. \<up>(r = app_s_f_v_s_mem_size ms i vs) *
+   mi \<mapsto>\<^sub>a mis * (list_assn mem_m_assn) ms mis * inst_m_assn (f_inst i) ii>"
+  unfolding app_s_f_v_s_mem_size_m_def inst_m_assn_def list_assn_conv_idx
+  apply extract_pre_pure
+  apply sep_auto
+  apply (extract_list_idx "inst.mems (f_inst i) ! 0")
+  apply (sep_auto)
+  apply (reinsert_list_idx "inst.mems (f_inst i) ! 0")
+  apply (sep_auto)
+  subgoal by (auto simp add: app_s_f_v_s_mem_size_def smem_ind_def mem_size_def mem_length_def mem_rep_length_def split: option.split list.split)  
+  apply (sep_auto)
+  done
+    
+find_theorems app_s_f_v_s_mem_size
+
+lemma run_step_b_e_m_run_step_b_e_Unreachable:
+  assumes "execute (run_step_b_e_m Unreachable cfg_m) h = Some ((cfg_m', res), h')"
+  shows "run_step_b_e Unreachable (config_m_to_config h cfg_m) = ((config_m_to_config h' cfg_m'), res)"
+  using assms
+  by (auto simp add: Heap_Monad.return_def Heap_Monad.heap_def config_m_to_config_def split: frame_context_m.splits frame_context.splits config_m.splits redex.splits prod.splits)
+
+lemma run_step_b_e_m_run_step_b_e:
+  assumes "execute (run_step_b_e_m b_e cfg_m) h = Some ((cfg_m', res), h')"
+  shows "run_step_b_e b_e (config_m_to_config h cfg_m) = ((config_m_to_config h' cfg_m'), res)"
+  using assms
+  sorry
+
+lemma run_step_e_m_run_step_e:
+  assumes "execute (run_step_e_m e cfg_m) h = Some ((cgf_m', res), h')"
+  shows "run_step_e e (config_m_to_config h cfg_m) = ((config_m_to_config h' cfg_m'), res)"
+  sorry
+
+lemma run_iter_m_run_iter:
+  assumes "execute (run_iter_m n cfg_m) h = Some ((cgf_m', res), h')"
+  shows "run_iter n (config_m_to_config h cfg_m) = ((config_m_to_config h' cfg_m'), res)"
+  sorry
 end
