libs/List_Assn.thy
@@ -1,0 +1,339 @@
+theory List_Assn
+imports "Separation_Logic_Imperative_HOL_Partial/Sep_Main" "HOL-Library.Rewrite"
+begin
+
+subsection "Lists"
+
+fun list_assn :: "('a \<Rightarrow> 'c \<Rightarrow> assn) \<Rightarrow> 'a list \<Rightarrow> 'c list \<Rightarrow> assn" where
+  "list_assn P [] [] = emp"
+| "list_assn P (a#as) (c#cs) = P a c * list_assn P as cs"
+| "list_assn _ _ _ = false"
+
+lemma list_assn_aux_simps[simp]:
+  "list_assn P [] l' = (\<up>(l'=[]))"
+  "list_assn P l [] = (\<up>(l=[]))"
+   apply (cases l')
+    apply simp
+   apply simp
+  apply (cases l)
+   apply simp
+  apply simp
+  done
+
+lemma list_assn_aux_append[simp]:
+  "length l1=length l1' \<Longrightarrow> 
+    list_assn P (l1@l2) (l1'@l2') 
+    = list_assn P l1 l1' * list_assn P l2 l2'"
+  apply (induct rule: list_induct2)
+   apply simp
+  apply (simp add: star_assoc)
+  done
+
+lemma list_assn_aux_ineq_len: "length l \<noteq> length li \<Longrightarrow> list_assn A l li = false"
+proof (induction l arbitrary: li)
+  case (Cons x l li) thus ?case by (cases li; auto)
+qed simp
+
+lemma list_assn_aux_append2[simp]:
+  assumes "length l2=length l2'"  
+  shows "list_assn P (l1@l2) (l1'@l2') 
+    = list_assn P l1 l1' * list_assn P l2 l2'"
+  apply (cases "length l1 = length l1'")
+   apply (erule list_assn_aux_append)
+  apply (simp add: list_assn_aux_ineq_len assms)
+  done
+
+lemma list_assn_simps[simp]:
+  "(list_assn P) [] [] = emp"
+  "(list_assn P) (a#as) (c#cs) = P a c * (list_assn P) as cs"
+  "(list_assn P) (a#as) [] = false"
+  "(list_assn P) [] (c#cs) = false"
+     apply simp_all
+  done
+
+
+lemma list_assn_mono: 
+  "\<lbrakk>\<And>x x'. P x x'\<Longrightarrow>\<^sub>AP' x x'\<rbrakk> \<Longrightarrow> list_assn P l l' \<Longrightarrow>\<^sub>A list_assn P' l l'"
+  apply (induct P l l' rule: list_assn.induct)
+  by (auto intro: ent_star_mono)
+
+lemma list_assn_cong[fundef_cong]:
+  assumes "xs=xs'" "xsi=xsi'"
+  assumes "\<And>x xi. x\<in>set xs' \<Longrightarrow> xi\<in>set xsi' \<Longrightarrow> A x xi = A' x xi"
+  shows "list_assn A xs xsi = list_assn A' xs' xsi'"  
+  using assms
+  apply (induct A\<equiv>A xs' xsi' arbitrary: xs xsi rule: list_assn.induct)
+     apply simp_all
+  done
+
+term prod_list
+
+
+definition "listI_assn I A xs xsi \<equiv> 
+    \<up>(length xsi=length xs \<and> I\<subseteq>{0..<length xs}) 
+  * Finite_Set.fold (\<lambda>i a. a * A (xs!i) (xsi!i)) 1 I"
+
+
+lemma aux: "Finite_Set.fold (\<lambda>i aa. aa * P ((a # as) ! i) ((c # cs) ! i)) emp {0..<Suc (length as)}
+  = P a c * Finite_Set.fold (\<lambda>i aa. aa * P (as ! i) (cs ! i)) emp {0..<length as}" 
+proof -
+  have 1: "{0..<Suc (length as)} = Set.insert 0 {1..<Suc (length as)}" by auto 
+
+  have 2: "{Suc 0..<Suc (Suc n)} = Set.insert (Suc n) {Suc 0 ..< Suc n}" for n by auto
+  have 3: "{0..<Suc n} = Set.insert n {0..<n}" for n by auto
+
+  have A: "
+    Finite_Set.fold P emp {Suc 0..<Suc n} 
+    = Finite_Set.fold Q emp {0..<n}" 
+    if "\<forall>i x. P (Suc i) x = Q i x"
+      and "comp_fun_commute P"
+      and "comp_fun_commute Q"
+    for P Q n
+    using that
+    apply (induction n arbitrary: a)
+    subgoal by simp
+    apply (simp add: comp_fun_commute.fold_insert)
+    apply (subst 2)
+    apply (subst 3)
+    apply (simp add: comp_fun_commute.fold_insert)
+    done 
+  show ?thesis
+    apply (simp add: 1)
+    apply (subst comp_fun_commute.fold_insert_remove)
+    subgoal
+      apply unfold_locales
+      apply (auto simp: fun_eq_iff algebra_simps)
+      done
+    subgoal by simp
+    apply simp
+    apply (rewrite at "\<hole> = _*_" mult.commute)
+    apply (rule arg_cong[where f="\<lambda>x. P _ _ * x"])
+    apply (rule A)
+    subgoal by auto
+    subgoal
+      apply unfold_locales
+      apply (auto simp: fun_eq_iff algebra_simps)
+      done
+    subgoal
+      apply unfold_locales
+      apply (auto simp: fun_eq_iff algebra_simps)
+      done
+    done
+qed    
+
+
+lemma list_assn_conv_idx: "list_assn A xs xsi = listI_assn {0..<length xs} A xs xsi"  
+  apply (induction A xs xsi rule: list_assn.induct)
+     apply (auto simp: listI_assn_def aux)
+  done
+
+lemma listI_assn_conv: "n=length xs \<Longrightarrow> listI_assn {0..<n} A xs xsi = list_assn A xs xsi"
+  by (simp add: list_assn_conv_idx)
+
+lemma listI_assn_conv': "n=length xs \<Longrightarrow> listI_assn {0..<n} A xs xsi *F  = list_assn A xs xsi* F"
+  by (simp add: list_assn_conv_idx)
+
+lemma listI_assn_finite[simp]: "\<not>finite I \<Longrightarrow> listI_assn I A xs xsi = false"
+  using subset_eq_atLeast0_lessThan_finite by (auto simp: listI_assn_def)
+
+
+find_theorems Finite_Set.fold name: cong  
+
+lemma mult_fun_commute: "comp_fun_commute (\<lambda>i (a::assn). a * f i)"
+  apply unfold_locales
+  apply (auto simp: fun_eq_iff mult_ac)
+  done
+
+lemma listI_assn_weak_cong: 
+  assumes I: "I=I'" "A=A'" "length xs=length xs'" "length xsi=length xsi'"
+  assumes A: "\<And>i. \<lbrakk>i\<in>I; i<length xs; length xs=length xsi \<rbrakk> 
+    \<Longrightarrow> xs!i = xs'!i \<and> xsi!i = xsi'!i"
+  shows "listI_assn I A xs xsi = listI_assn I' A' xs' xsi'"
+  unfolding listI_assn_def
+  apply (simp add: I)
+  apply (cases "length xsi' = length xs' \<and> I' \<subseteq> {0..<length xs'}"; simp only:; simp)
+  apply (rule Finite_Set.fold_cong)
+       apply (simp_all add: mult_fun_commute)
+  subgoal by (meson subset_eq_atLeast0_lessThan_finite)
+  subgoal using A by (auto simp: fun_eq_iff I)
+  done
+
+lemma listI_assn_cong: 
+  assumes I: "I=I'" "length xs=length xs'" "length xsi=length xsi'"
+  assumes A: "\<And>i. \<lbrakk>i\<in>I; i<length xs; length xs=length xsi \<rbrakk> 
+    \<Longrightarrow> xs!i = xs'!i \<and> xsi!i = xsi'!i 
+      \<and> A (xs!i) (xsi!i) = A' (xs'!i) (xsi'!i)"
+  shows "listI_assn I A xs xsi = listI_assn I' A' xs' xsi'"
+  unfolding listI_assn_def
+  apply (simp add: I)
+  apply (cases "length xsi' = length xs' \<and> I' \<subseteq> {0..<length xs'}"; simp only:; simp)
+  apply (rule Finite_Set.fold_cong)
+       apply (simp_all add: mult_fun_commute)
+  subgoal by (meson subset_eq_atLeast0_lessThan_finite)
+  subgoal using A by (fastforce simp: fun_eq_iff I)
+  done
+
+
+
+lemma listI_assn_insert: "i\<notin>I \<Longrightarrow> i<length xs \<Longrightarrow> 
+       listI_assn (Set.insert i I) A xs xsi = A (xs!i) (xsi!i) * listI_assn I A xs xsi"
+  apply (cases "finite I"; simp?)
+  unfolding listI_assn_def
+  apply (subst comp_fun_commute.fold_insert)
+  subgoal 
+    apply unfold_locales
+    apply (auto simp: fun_eq_iff algebra_simps)
+    done
+  subgoal by simp  
+  subgoal by simp  
+  subgoal by (auto simp: algebra_simps)
+  done
+
+lemma listI_assn_extract:
+  assumes "i\<in>I" "i<length xs"  
+  shows "listI_assn I A xs xsi = A (xs!i) (xsi!i) * listI_assn (I-{i}) A xs xsi"  
+proof -
+  have 1: "I = Set.insert i (I-{i})" using assms by auto 
+  show ?thesis
+    apply (subst 1)
+    apply (subst listI_assn_insert)
+    using assms by auto
+qed    
+
+
+lemma listI_assn_reinsert:
+  assumes "P \<Longrightarrow>\<^sub>A A (xs!i) (xsi!i) * listI_assn (I-{i}) A xs xsi * F"
+  assumes "i<length xs" "i\<in>I"
+  assumes "listI_assn I A xs xsi * F \<Longrightarrow>\<^sub>A Q"
+  shows "P \<Longrightarrow>\<^sub>A Q"
+proof -
+  show ?thesis
+    apply (rule ent_trans[OF assms(1)])
+    apply (subst listI_assn_extract[symmetric])
+    subgoal by fact
+    subgoal by fact
+    subgoal by fact
+    done
+qed  
+
+lemma listI_assn_reinsert_upd:
+  fixes xs xsi :: "_ list"
+  assumes "P \<Longrightarrow>\<^sub>A A x xi * listI_assn (I-{i}) A xs xsi * F"
+  assumes "i<length xs" "i\<in>I"
+  assumes "listI_assn I A (xs[i:=x]) (xsi[i:=xi]) * F \<Longrightarrow>\<^sub>A Q"
+  shows "P \<Longrightarrow>\<^sub>A Q"
+proof (cases "length xs = length xsi")
+  case True
+  have 1: "listI_assn (I-{i}) A xs xsi = listI_assn (I-{i}) A (xs[i:=x]) (xsi[i:=xi])"
+    by (rule listI_assn_cong) auto
+
+  have 2: "A x xi = A ((xs[i:=x])!i) ((xsi[i:=xi])!i)" using \<open>i<length xs\<close> True by auto
+
+  from assms[unfolded 1 2] show ?thesis 
+    apply (rule_tac listI_assn_reinsert)
+       apply assumption
+      apply simp_all
+    done
+
+next    
+  case False
+  with assms(1) have "P \<Longrightarrow>\<^sub>A false"
+    by (simp add: listI_assn_def)
+  thus ?thesis using ent_false_iff entailsI by blast  
+qed  
+
+
+lemma listI_assn_reinsert':
+  assumes "P \<Longrightarrow>\<^sub>A A (xs!i) (xsi!i) * listI_assn (I-{i}) A xs xsi * F"
+  assumes "i<length xs" "i\<in>I"
+  assumes "<listI_assn I A xs xsi * F>c<Q>"
+  shows "<P>c<Q>"
+proof -
+  show ?thesis
+    apply (rule cons_pre_rule[OF assms(1)])
+    apply (subst listI_assn_extract[symmetric])
+    subgoal by fact
+    subgoal by fact
+    subgoal by fact
+    done
+qed  
+
+lemma listI_assn_reinsert_upd':
+  fixes xs xsi :: "_ list"
+  assumes "P \<Longrightarrow>\<^sub>A A x xi * listI_assn (I-{i}) A xs xsi * F"
+  assumes "i<length xs" "i\<in>I"
+  assumes "<listI_assn I A (xs[i:=x]) (xsi[i:=xi]) * F> c <Q>"
+  shows "<P> c <Q>"
+  by (meson assms(1) assms(2) assms(3) assms(4) cons_pre_rule ent_refl listI_assn_reinsert_upd)
+
+
+
+definition "unwrap_list_idxs (xsi::_::heap list) \<equiv> return ()" (* list_assn \<rightarrow> list_assnI *)
+definition "wrap_list_idxs (xsi::_::heap list) \<equiv> return ()" (* list_assnI \<rightarrow> list_assn *)
+
+definition "extract_list_idx (xsi::_::heap list) (i::nat) \<equiv> return ()" (* list_assnI _ A \<rightarrow> A (xs!i) (xsi!i) * \<dots> *)
+definition "reinsert_list_idx (xsi::_::heap list) (i::nat) \<equiv> return ()" (* A (xs!i) (xsi!i) * \<dots> \<rightarrow> list_assnI _ A *)
+
+lemma unwrap_list_idxs_rule[sep_heap_rules]: 
+  "<list_assn A xs xsi> unwrap_list_idxs xsi <\<lambda>_. listI_assn {0..<length xs} A xs xsi>"
+  unfolding unwrap_list_idxs_def
+  by (sep_auto simp: list_assn_conv_idx)
+
+lemma wrap_list_idxs_rule[sep_heap_rules]:
+  "I={0..<length xs} \<Longrightarrow> <listI_assn I A xs xsi> wrap_list_idxs xsi <\<lambda>_. list_assn A xs xsi>"
+  unfolding wrap_list_idxs_def
+  by (sep_auto simp: list_assn_conv_idx)
+
+lemma extract_list_idx_rule[sep_heap_rules]:
+  "i\<in>I \<Longrightarrow> <listI_assn I A xs xsi> extract_list_idx xsi i <\<lambda>_. A (xs!i) (xsi!i) * listI_assn (I-{i}) A xs xsi>"
+  unfolding extract_list_idx_def
+  apply sep_auto 
+    (* TODO: Cleaner proof. listI_assn implies that index set is <length! *)
+  by (smt (verit, best) atLeastLessThan_iff ent_false ent_refl insert_absorb insert_subset 
+      listI_assn_def listI_assn_extract pure_false star_false_left)
+
+lemma reinsert_list_idx_rule[sep_heap_rules]:
+  "i\<notin>I \<Longrightarrow> i<length xs \<Longrightarrow> <A (xs!i) (xsi!i) * listI_assn I A xs xsi> reinsert_list_idx xsi i <\<lambda>_. listI_assn (Set.insert i I) A xs xsi>"
+  unfolding reinsert_list_idx_def
+  apply sep_auto
+  by (simp add: listI_assn_insert)
+
+
+
+
+
+lemma subst_not_in: 
+  assumes "i\<notin>I " " i<length xs "
+  shows "listI_assn I A (xs[i:=x1]) (xsi[i := x2]) = listI_assn I A xs xsi"
+  apply (rule listI_assn_cong)
+  using assms
+  by (auto simp add: nth_list_update')
+
+lemma listI_assn_subst: 
+  assumes "i\<notin>I "" i<length xs "
+  shows "listI_assn (Set.insert i I) A (xs[i:=x1]) (xsi[i := x2]) = A x1 x2 * listI_assn I A xs xsi" 
+  by (smt (z3) assms(1) assms(2) length_list_update listI_assn_def listI_assn_insert nth_list_update_eq pure_false star_false_left star_false_right subst_not_in)
+
+
+(* TODO: Move *)  
+lemma mod_starE: assumes "h \<Turnstile> a*b" obtains h\<^sub>1 h\<^sub>2 where "h\<^sub>1 \<Turnstile> a" "h\<^sub>2 \<Turnstile> b"
+  using assms by (auto dest: mod_starD)
+
+named_theorems extract_pure_rules  
+  
+lemma extract_pre_list_assn_lengthD[extract_pure_rules]: "h \<Turnstile> list_assn A xs xsi \<Longrightarrow> length xsi = length xs"
+  by (metis list_assn_aux_ineq_len mod_false)
+  
+lemma extract_pre_listI_assn_lengthD[extract_pure_rules]: "h \<Turnstile> listI_assn I A xs xsi \<Longrightarrow> length xsi = length xs"
+  by (simp add: listI_assn_def)
+  
+
+method extract_pre_pure uses dest =
+  (rule hoare_triple_preI | drule asm_rl[of "_\<Turnstile>_"]),
+  (determ \<open>elim mod_starE dest[elim_format] extract_pure_rules[elim_format]\<close>)?,
+  ((determ \<open>thin_tac "_ \<Turnstile> _"\<close>)+)?,
+  (simp (no_asm) only: triv_forall_equality)?
+
+
+
+end
